\begin{aligned} y=y(x, t) &=A e^{i \theta} \\ &=A(\cos \theta+i \sin \theta) \\ &=A(\cos (k x-\omega t)+i \sin (k x-\omega t)) \\ &=A \cos (k x-\omega t)+i A \sin (k x-\omega t) \\ &=A \cos \left(\frac{2 \pi}{\lambda} x-\frac{2 \pi v}{\lambda} t\right)+i A \sin \left(\frac{2 \pi}{\lambda} x-\frac{2 \pi v}{\lambda} t\right) \\ &=A \cos \frac{2 \pi}{\lambda}(x-v t)+i A \sin \frac{2 \pi}{\lambda}(x-v t) \end{aligned}  
  
  
$\begin{aligned} y=y(x, t) &=A e^{i \theta} \\ &=A(\cos \theta+i \sin \theta) \\ &=A(\cos (k x-\omega t)+i \sin (k x-\omega t)) \\ &=A \cos (k x-\omega t)+i A \sin (k x-\omega t) \\ &=A \cos \left(\frac{2 \pi}{\lambda} x-\frac{2 \pi v}{\lambda} t\right)+i A \sin \left(\frac{2 \pi}{\lambda} x-\frac{2 \pi v}{\lambda} t\right) \\ &=A \cos \frac{2 \pi}{\lambda}(x-v t)+i A \sin \frac{2 \pi}{\lambda}(x-v t) \end{aligned}$  


$$
\begin{aligned} y=y(x, t) &=A e^{i \theta} \\ &=A(\cos \theta+i \sin \theta) \\ &=A(\cos (k x-\omega t)+i \sin (k x-\omega t)) \\ &=A \cos (k x-\omega t)+i A \sin (k x-\omega t) \\ &=A \cos \left(\frac{2 \pi}{\lambda} x-\frac{2 \pi v}{\lambda} t\right)+i A \sin \left(\frac{2 \pi}{\lambda} x-\frac{2 \pi v}{\lambda} t\right) \\ &=A \cos \frac{2 \pi}{\lambda}(x-v t)+i A \sin \frac{2 \pi}{\lambda}(x-v t) \end{aligned}
$$  


\begin{equation}
\begin{aligned} y=y(x, t) &=A e^{i \theta} \\ &=A(\cos \theta+i \sin \theta) \\ &=A(\cos (k x-\omega t)+i \sin (k x-\omega t)) \\ &=A \cos (k x-\omega t)+i A \sin (k x-\omega t) \\ &=A \cos \left(\frac{2 \pi}{\lambda} x-\frac{2 \pi v}{\lambda} t\right)+i A \sin \left(\frac{2 \pi}{\lambda} x-\frac{2 \pi v}{\lambda} t\right) \\ &=A \cos \frac{2 \pi}{\lambda}(x-v t)+i A \sin \frac{2 \pi}{\lambda}(x-v t) \end{aligned}
\end{equation}
